\include{"../preamble.tex"}
%\documentclass[12pt]{article}
%\title{ECE C143A Homework 6}
%\usepackage{subcaption}
%\author{Lawrence Liu}
%\usepackage{graphicx}
%\usepackage{amsmath}
%\usepackage{pdfpages}
%\newcommand{\Laplace}{\mathscr{L}}
%\setlength{\parskip}{\baselineskip}%
%\setlength{\parindent}{0pt}%
%\usepackage{xcolor}
%\usepackage{listings}
%\definecolor{backcolour}{rgb}{0.95,0.95,0.92}
%\usepackage{amssymb}
%\lstdefinestyle{mystyle}{
%    backgroundcolor=\color{backcolour}}
%\lstset{style=mystyle}
\title{ECE 231A HW 1}
\begin{document}
\maketitle
\section*{Problem 3}
\subsection*{(a)}
The entropy of $H(X)$ is
$$H(X)=-\sum_{x\in X} p(x)\log\left(p(x)\right)$$
and we have that
\begin{align*}
	H(X|Y)&=\sum_{x\in X, y \in Y} p(y)H(X|Y=y)\\
	&=\left(\sum_{x\in S}p(x)\right)H(X|Y=1)+\left(\sum_{x\notin S}p(x)\right)H(X|Y=0)
\end{align*}
We have
\begin{align*}
	H(X|Y=1)&=-\sum_{x\in S}p(x|Y=1)\log(p(x|Y=1))\\
	&=-\sum_{x\in S}\frac{p(x)}{\sum_{x\in S}p(x)}\log\left(\frac{p(x)}{\sum_{x\in S}p(x)}\right)
\end{align*}
likewise we have
\begin{align*}
	H(X|Y=0)&=-\sum_{x\notin S}p(x|Y=0)\log(p(x|Y=0))\\
	&=-\sum_{x\notin S}\frac{p(x)}{\sum_{x\notin S}p(x)}\log\left(\frac{p(x)}{\sum_{x\notin S}p(x)}\right)
\end{align*}
Therefore we have
\begin{align*}
	H(X|Y)&=-\sum_{x\in S}p(x)\left(\log(p(x))-\log\left(
		\sum_{x\in S}p(x)
	\right)\right)-\sum_{x\notin S}p(x)\left(\log(p(x))-\log\left(
		\sum_{x\notin S}p(x)
	\right)\right)\\
	&=H(X)+\sum_{x\in S}p(x)\log\left(
		\sum_{x\in S}p(x)
	\right)+\sum_{x\notin S}p(x)\log\left(
		\sum_{x\notin S}p(x)
	\right)
\end{align*}
Therefore we have
$$H(X)-H(X|Y)=\boxed{-\sum_{x\in S}p(x)\log\left(
	\sum_{x\in S}p(x)
\right)-\sum_{x\notin S}p(x)\log\left(
	\sum_{x\notin S}p(x)
\right)}$$
\subsection*{(b)}
$H(X)-H(X|Y)$ is maximized when 
$\sum_{x\in S}p(x)=\sum_{x\notin S}p(x)=\frac{1}{2}$, this is possible
when $S=\boxed{2,5}$ or $S=\boxed{1,2,4}$
\section*{Problem 6}
\subsection*{(a)}
\begin{align*}
	H(x)&=-\sum_{x\in X} p(x)\log(p(x))\\
	&=p(A)\log(p(A))+p(B)\log(p(B))+p(C)\log(p(C))\\&+p(D)\log(p(D))+p(E)\log(p(E))+p(F)\log(p(F))\\
	&=\frac{1}{2}\log(4)+\frac{1}{4}\log(8)+\frac{3}{16}\log(\frac{16}{3})+\frac{1}{16}\log(16)\\
	&=\boxed{2.2452\text{ shannons}}
\end{align*}
\end{document}
