\include{"../preamble.tex"}
\title{ECE 231A Project 3 Part 2}
\begin{document}
\maketitle
\section*{Problem 1}
We can rewrite $P(l(x)<l'(x))>P(l(x)>l'(x))$ as
\begin{align*}
    \sum_{x} p(x)sign(l(x)-l'(x))&\leq 0
\end{align*}
using the identity $sign(a-b)\leq D^t-1$, we get
\begin{align*}
    \sum_{x} p(x)sign(l(x)-l'(x))&\leq \sum_{x} p(x)\left(D^{l(x)-l'(x)}+1\right)\\
    &=\sum_{x}D^{l'(x)}-1
\end{align*}
From the kraft inequality, we then get that $\sum_{x}D^{l'(x)}\leq 1$.
and thus we get that $\sum_{x}D^{l'(x)}-1\leq 0$.
\section*{Problem 2}
\subsection*{(a)}
let $l'(x)=-\log(q(x))$, then we have
\begin{align*}
    p(l'(x)\leq l^*(x)-\gamma)&=p(-\log_D(q(x))\leq -\log_D(p(x))-\gamma)\\
    &=p(q(x)\geq p(x)D^{\gamma})\\
    &=\sum_{x:p(x)D^{\gamma}\leq q(x)}p(x)\\
    &\leq \sum_{x:p(x)D^{\gamma}\leq q(x)}q(x)D^{-\gamma}\\
    &=\sum_{x}q(x)D^{-\gamma}\\
    &=D^{-\gamma}
\end{align*} 
Thus we get
$$
    p(l'(x)\leq l^*(x)-\gamma)\leq |D|^{-\gamma}$$   
\subsection*{(b)}
We have 
\begin{align*}
    p(l(x)>l'(x)+1)&=p\left(\lceil \log_D\left(\frac{1}{p(x)}\right)\rceil >l'(x)+1\right)\\
    &\leq p(1-log_D(p(x))>l'(x)+1)\\
    &=\leq p(-\log_D(p(x))<l'(x))
\end{align*}
Since $l(x)$ must be an integer we have that this is equal to 
$$p(-\log_D(p(x))<l'(x))=p(l'(x)\leq-\log_D(p(x))-1)$$
from part (a) we know that 
$$p(l'(x)\leq-\log_D(p(x))-1)\leq D^{-1}\leq \frac{1}{2}$$
since $D\geq 2$. thus we have that 
$$p(l(x)>l'(x)+1)\leq \frac{1}{2}$$
and thus 
$$p(l(x)>l'(x)+1)\leq p(l(x)\leq l'(x)+1)$$

\end{document}
